base cases

dp/6_2.dfy
@@ -16,13 +16,13 @@ module SixTwo {
     predicate a1(miles: seq<nat>)
     requires |miles|>0 ==> miles[0] == 0
     {
-        a2(miles)
+        |miles|>0 ==> a2(miles)
     }
 
     // Distances are strictly increasing.
     predicate a2(miles: seq<nat>)
     {
-        forall i,j :: 0 <= i < j < |miles| 
+        forall i,j :: 0 <= i <= j < |miles| 
             ==> miles[i] < miles[j]
     }
 
@@ -34,17 +34,24 @@ module SixTwo {
 
     // Min. function to serve as our recurrence.
     function a4(miles: seq<nat>, i: nat): nat
-    requires 0 <= i < |miles|
+    requires |miles|==0 ==> i==0
     requires |miles|==1 ==> i==|miles|-1
+    requires |miles|>0 ==> 0 <= i < |miles|
     {
         if |miles|==0 then 0 else
         if |miles|==1 then miles[i] else 
         0
     }
 
-/*
     method Main()
     {
+        // Base cases.
+        var m0 :seq<nat> := [];
+        assert a1(m0);
+        assert a4(m0, 0) == 0;
+
+        var m1 := [0];
+        assert a1(m0);
+        assert a4(m0, |m1|-1) == 0;
     }
-*/
 }
